Thread ids

theories/bi/weakestpre.v
@@ -1,6 +1,8 @@
 From stdpp Require Export coPset.
 From iris.bi Require Import interface derived_connectives.
 From diris.program_logic Require Import language.
+From diris.program_logic Require Import ectx_language.
+
 
 Inductive stuckness := NotStuck | MaybeStuck.
 
@@ -27,12 +29,12 @@ and [s] to be [NotStuck] or [MaybeStuck].  This will fail to typecheck if [A] is
 not [stuckness].  If we ever want to use the notation [WP e @ E {{ Φ }}] with a
 different [A], the plan is to generalize the notation to use [Inhabited] instead
 to pick a default value depending on [A]. *)
-Class Wp (Λ : language) (PROP A : Type) :=
+Class Wp (Λ : ectxLanguage) (PROP A : Type) :=
   wp : A → coPset → expr Λ → (val Λ → PROP) → PROP.
 Arguments wp {_ _ _ _} _ _ _%E _%I.
 Instance: Params (@wp) 7 := {}.
 
-Class Twp (Λ : language) (PROP A : Type) :=
+Class Twp (Λ : ectxLanguage) (PROP A : Type) :=
   twp : A → coPset → expr Λ → (val Λ → PROP) → PROP.
 Arguments twp {_ _ _ _} _ _ _%E _%I.
 Instance: Params (@twp) 7 := {}.
