theories/program_logic/adequacy.v
@@ -6,7 +6,7 @@ Set Default Proof Using "Type".
 Import uPred.
 
 (** This file contains the adequacy statements of the Iris program logic. First
-we prove a number of auxilary results. *)
+we prove a number of auxiliary results. *)
 Section adequacy.
 Context `{!irisG Λ Σ}.
 Implicit Types e : expr Λ.
@@ -14,48 +14,57 @@ Implicit Types P Q : iProp Σ.
 Implicit Types Φ : val Λ → iProp Σ.
 Implicit Types Φs : list (val Λ → iProp Σ).
 
-Notation wptp s t := ([∗ list] ef ∈ t, WP ef @ s; ⊤ {{ fork_post }})%I.
+Notation wptp s j t := ([∗ list] i ↦ ef ∈ t, WP ef @ (s,j+i); ⊤ {{ fork_post }})%I.
 
-Lemma wp_step s e1 σ1 κ κs e2 σ2 efs m Φ :
+Lemma wp_step s i e1 σ1 κ κs e2 σ2 efs es Φ :
+  es !! i = Some e1 →
   prim_step e1 σ1 κ e2 σ2 efs →
-  state_interp σ1 (κ ++ κs) m -∗ WP e1 @ s; ⊤ {{ Φ }} ={⊤,∅}▷=∗
-  state_interp σ2 κs (length efs + m) ∗ WP e2 @ s; ⊤ {{ Φ }} ∗ wptp s efs.
+  state_interp σ1 (κ ++ κs) es -∗ WP e1 @ (s,i); ⊤ {{ Φ }} ={⊤,∅}▷=∗
+  state_interp σ2 κs (<[i:=e2]> es ++ efs) ∗ WP e2 @ (s,i); ⊤ {{ Φ }} ∗ wptp s (length es) efs.
 Proof.
-  rewrite {1}wp_unfold /wp_pre. iIntros (?) "Hσ H".
+  rewrite {1}wp_unfold /wp_pre. iIntros (??) "Hσ H".
   rewrite (val_stuck e1 σ1 κ e2 σ2 efs) //.
-  iMod ("H" $! σ1 with "Hσ") as "(_ & H)".
+  iMod ("H" $! σ1 _ _ _ empty_ectx with "[%] Hσ") as "(_ & H)".
+  { by rewrite fill_empty. }
   iMod ("H" $! e2 σ2 efs with "[//]") as "H".
+  rewrite fill_empty.
   by iIntros "!> !>".
 Qed.
 
 Lemma wptp_step s e1 t1 t2 κ κs σ1 σ2 Φ :
   step (e1 :: t1,σ1) κ (t2, σ2) →
-  state_interp σ1 (κ ++ κs) (length t1) -∗ WP e1 @ s; ⊤ {{ Φ }} -∗ wptp s t1 ==∗
+  state_interp σ1 (κ ++ κs) (e1 :: t1) -∗ WP e1 @ (s,0); ⊤ {{ Φ }} -∗ wptp s 1 t1 ==∗
   ∃ e2 t2', ⌜t2 = e2 :: t2'⌝ ∗
-  |={⊤,∅}▷=> state_interp σ2 κs (pred (length t2)) ∗ WP e2 @ s; ⊤ {{ Φ }} ∗ wptp s t2'.
+  |={⊤,∅}▷=> state_interp σ2 κs t2 ∗ WP e2 @ (s,0); ⊤ {{ Φ }} ∗ wptp s 1 t2'.
 Proof.
   iIntros (Hstep) "Hσ He Ht".
   destruct Hstep as [e1' σ1' e2' σ2' efs [|? t1'] t2' ?? Hstep]; simplify_eq/=.
   - iExists e2', (t2' ++ efs). iModIntro. iSplitR; first by eauto.
-    iMod (wp_step with "Hσ He") as "H"; first done.
+    iMod (wp_step with "Hσ He") as "H"; [done..|].
     iIntros "!> !>". iMod "H" as "(Hσ & He2 & Hefs)".
-    iIntros "!>". rewrite Nat.add_comm app_length. iFrame.
+    iIntros "!>". iFrame.
   - iExists e, (t1' ++ e2' :: t2' ++ efs); iSplitR; first eauto.
     iFrame "He". iDestruct "Ht" as "(Ht1 & He1 & Ht2)".
-    iModIntro. iMod (wp_step with "Hσ He1") as "H"; first done.
+    iModIntro. iMod (wp_step with "Hσ He1") as "H". 
+    { by rewrite Nat.add_0_r /= lookup_app_r // Nat.sub_diag. }
+    { done. }
     iIntros "!> !>". iMod "H" as "(Hσ & He2 & Hefs)". iIntros "!>".
-    rewrite !app_length /= !app_length.
-    replace (length t1' + S (length t2' + length efs))
-      with (length efs + (length t1' + S (length t2'))) by omega. iFrame.
+    iSplitL "Hσ".
+    { by rewrite Nat.add_0_r /= insert_app_r_alt // Nat.sub_diag /= -assoc_L. }
+    iFrame "Ht1 Ht2 He2". simpl.
+    iApply (big_sepL_impl with "Hefs").
+    iModIntro. iIntros.
+    by rewrite !app_length /= !Nat.add_succ_r !Nat.add_assoc /=.
 Qed.
 
+
 Lemma wptp_steps s n e1 t1 κs κs' t2 σ1 σ2 Φ :
-  nsteps n (e1 :: t1, σ1) κs (t2, σ2) →
-  state_interp σ1 (κs ++ κs') (length t1) -∗ WP e1 @ s; ⊤ {{ Φ }} -∗ wptp s t1
+  language.nsteps n (e1 :: t1, σ1) κs (t2, σ2) →
+  state_interp σ1 (κs ++ κs') (e1 :: t1) -∗ WP e1 @ (s,0); ⊤ {{ Φ }} -∗ wptp s 1 t1
   ={⊤,∅}▷=∗^n ∃ e2 t2',
     ⌜t2 = e2 :: t2'⌝ ∗
-    state_interp σ2 κs' (pred (length t2)) ∗
-    WP e2 @ s; ⊤ {{ Φ }} ∗ wptp s t2'.
+    state_interp σ2 κs' t2 ∗
+    WP e2 @ (s,0); ⊤ {{ Φ }} ∗ wptp s 1 t2'.
 Proof.
   revert e1 t1 κs κs' t2 σ1 σ2; simpl.
   induction n as [|n IH]=> e1 t1 κs κs' t2 σ1 σ2 /=.
@@ -67,48 +76,54 @@ Proof.
   by iApply (IH with "Hσ He Ht").
 Qed.
 
-Lemma wp_not_stuck κs m e σ Φ :
-  state_interp σ κs m -∗ WP e {{ Φ }} ={⊤}=∗ ⌜not_stuck e σ⌝.
+Lemma wp_not_stuck κs es e σ Φ i :
+  es !! i = Some e ->
+  state_interp σ κs es -∗ WP e @ (NotStuck,i); ⊤ {{ Φ }} ={⊤}=∗ ⌜not_stuck e σ⌝.
 Proof.
-  rewrite wp_unfold /wp_pre /not_stuck. iIntros "Hσ H".
+  rewrite wp_unfold /wp_pre /not_stuck. iIntros (?) "Hσ H".
   destruct (to_val e) as [v|] eqn:?; first by eauto.
-  iSpecialize ("H" $! σ [] κs with "Hσ"). rewrite sep_elim_l.
+  iSpecialize ("H" $! σ [] κs _ empty_ectx with "[%] Hσ").
+  { by rewrite fill_empty. }
+  rewrite sep_elim_l.
   iMod (fupd_plain_mask with "H") as %?; eauto.
 Qed.
 
 Lemma wptp_strong_adequacy Φ κs' s n e1 t1 κs t2 σ1 σ2 :
-  nsteps n (e1 :: t1, σ1) κs (t2, σ2) →
-  state_interp σ1 (κs ++ κs') (length t1) -∗
-  WP e1 @ s; ⊤ {{ Φ }} -∗
-  wptp s t1 ={⊤,∅}▷=∗^(S n) ∃ e2 t2',
+  language.nsteps n (e1 :: t1, σ1) κs (t2, σ2) →
+  state_interp σ1 (κs ++ κs') (e1 :: t1) -∗
+  WP e1 @ (s,0); ⊤ {{ Φ }} -∗
+  wptp s 1 t1 ={⊤,∅}▷=∗^(S n) ∃ e2 t2',
     ⌜ t2 = e2 :: t2' ⌝ ∗
-    ⌜ ∀ e2, s = NotStuck → e2 ∈ t2 → (is_Some (to_val e2) ∨ reducible e2 σ2 ∨ waiting e2 σ2) ⌝ ∗
-    state_interp σ2 κs' (length t2') ∗
+    ⌜ ∀ e2, s = NotStuck → e2 ∈ t2 → not_stuck e2 σ2 ⌝ ∗
+    state_interp σ2 κs' t2 ∗
     from_option Φ True (to_val e2) ∗
-    ([∗ list] v ∈ omap to_val t2', fork_post v).
+    ([∗ list] e ∈ t2', from_option fork_post True (to_val e)).
 Proof.
   iIntros (Hstep) "Hσ He Ht". rewrite Nat_iter_S_r.
   iDestruct (wptp_steps with "Hσ He Ht") as "Hwp"; first done.
   iApply (step_fupdN_wand with "Hwp").
   iDestruct 1 as (e2' t2' ?) "(Hσ & Hwp & Ht)"; simplify_eq/=.
   iMod (fupd_plain_keep_l ⊤
-    ⌜ ∀ e2, s = NotStuck → e2 ∈ (e2' :: t2') → (is_Some (to_val e2) ∨ reducible e2 σ2 ∨ waiting e2 σ2) ⌝%I
-    (state_interp σ2 κs' (length t2') ∗ WP e2' @ s; ⊤ {{ v, Φ v }} ∗ wptp s t2')%I
+    ⌜ ∀ e2, s = NotStuck → e2 ∈ (e2' :: t2') → not_stuck e2 σ2 ⌝%I
+    (state_interp σ2 κs' (e2' :: t2') ∗ WP e2' @ (s,0); ⊤ {{ v, Φ v }} ∗ wptp s 1 t2')%I
     with "[$Hσ $Hwp $Ht]") as "(Hsafe&Hσ&Hwp&Hvs)".
   { iIntros "(Hσ & Hwp & Ht)" (e' -> He').
     apply elem_of_cons in He' as [<-|(t1''&t2''&->)%elem_of_list_split].
     - iMod (wp_not_stuck with "Hσ Hwp") as "$"; auto.
-    - iDestruct "Ht" as "(_ & He' & _)". by iMod (wp_not_stuck with "Hσ He'"). }
+    - iDestruct "Ht" as "(_ & He' & _)". rewrite Nat.add_0_r /=.
+      iApply (wp_not_stuck with "Hσ He'").
+      by rewrite /= lookup_app_r // Nat.sub_diag. }
   iApply step_fupd_fupd. iApply step_fupd_intro; first done. iNext.
   iExists _, _. iSplitL ""; first done. iFrame "Hsafe Hσ".
   iSplitL "Hwp".
   - destruct (to_val e2') as [v2|] eqn:He2'; last done.
     apply of_to_val in He2' as <-. iApply (wp_value_inv' with "Hwp").
-  - clear Hstep. iInduction t2' as [|e t2'] "IH"; csimpl; first by iFrame.
-    iDestruct "Hvs" as "[Hv Hvs]". destruct (to_val e) as [v|] eqn:He.
-    + apply of_to_val in He as <-. iMod (wp_value_inv' with "Hv") as "$".
-      by iApply "IH".
-    + by iApply "IH".
+  - clear Hstep.
+    iApply big_sepL_fupd.
+    iApply (big_sepL_impl with "Hvs").
+    iIntros "!>" (i e ?) "He /=".
+    destruct (to_val e) as [v|] eqn:He; last by auto.
+    apply of_to_val in He as <-. iApply (wp_value_inv' with "He").
 Qed.
 End adequacy.
 
@@ -117,29 +132,29 @@ Theorem wp_strong_adequacy Σ Λ `{!invPreG Σ} e1 σ1 n κs t2 σ2 φ :
   (∀ `{Hinv : !invG Σ},
      (|={⊤}=> ∃
          (s: stuckness)
-         (stateI : state Λ → list (observation Λ) → nat → iProp Σ)
+         (stateI : state Λ → list (observation Λ) → list (expr Λ) → iProp Σ)
          (Φ fork_post : val Λ → iProp Σ),
        let _ : irisG Λ Σ := IrisG _ _ Hinv stateI fork_post in
-       stateI σ1 κs 0 ∗
-       WP e1 @ s; ⊤ {{ Φ }} ∗
+       stateI σ1 κs [e1] ∗
+       WP e1 @ (s,0); ⊤ {{ Φ }} ∗
        (∀ e2 t2',
          (* e2 is the final state of the main thread, t2' the rest *)
          ⌜ t2 = e2 :: t2' ⌝ -∗
          (* If this is a stuck-free triple (i.e. [s = NotStuck]), then all
          threads in [t2] are either done (a value) or reducible *)
-         ⌜ ∀ e2, s = NotStuck → e2 ∈ t2 → (is_Some (to_val e2) ∨ reducible e2 σ2 ∨ waiting e2 σ2) ⌝ -∗
+         ⌜ ∀ e2, s = NotStuck → e2 ∈ t2 → not_stuck e2 σ2 ⌝ -∗
          (* The state interpretation holds for [σ2] *)
-         stateI σ2 [] (length t2') -∗
+         stateI σ2 [] (e2 :: t2') -∗
          (* If the main thread is done, its post-condition [Φ] holds *)
          from_option Φ True (to_val e2) -∗
          (* For all threads that are done, their postcondition [fork_post] holds. *)
-         ([∗ list] v ∈ omap to_val t2', fork_post v) -∗
+         ([∗ list] e ∈ t2', from_option fork_post True (to_val e)) -∗
          (* Under all these assumptions, and while opening all invariants, we
          can conclude [φ] in the logic. After opening all required invariants,
          one can use [fupd_intro_mask'] or [fupd_mask_weaken] to introduce the
          fancy update. *)
          |={⊤,∅}=> ⌜ φ ⌝))%I) →
-  nsteps n ([e1], σ1) κs (t2, σ2) →
+  language.nsteps n ([e1], σ1) κs (t2, σ2) →
   (* Then we can conclude [φ] at the meta-level. *)
   φ.
 Proof.
@@ -165,14 +180,14 @@ Record adequate {Λ} (s : stuckness) (e1 : expr Λ) (σ1 : state Λ)
   adequate_not_stuck t2 σ2 e2 :
    s = NotStuck →
    rtc erased_step ([e1], σ1) (t2, σ2) →
-   e2 ∈ t2 → not_stuck e2 σ2 ∨ waiting e2 σ2
+   e2 ∈ t2 → not_stuck e2 σ2
 }.
 
 Lemma adequate_alt {Λ} s e1 σ1 (φ : val Λ → state Λ → Prop) :
   adequate s e1 σ1 φ ↔ ∀ t2 σ2,
     rtc erased_step ([e1], σ1) (t2, σ2) →
       (∀ v2 t2', t2 = of_val v2 :: t2' → φ v2 σ2) ∧
-      (∀ e2, s = NotStuck → e2 ∈ t2 → not_stuck e2 σ2 ∨ waiting e2 σ2).
+      (∀ e2, s = NotStuck → e2 ∈ t2 → not_stuck e2 σ2).
 Proof. split. intros []; naive_solver. constructor; naive_solver. Qed.
 
 (*
@@ -199,11 +214,11 @@ Corollary wp_adequacy Σ Λ `{!invPreG Σ} s e σ φ :
          (stateI : state Λ → list (observation Λ) → iProp Σ)
          (fork_post : val Λ → iProp Σ),
        let _ : irisG Λ Σ := IrisG _ _ Hinv (λ σ κs _, stateI σ κs) fork_post in
-       stateI σ κs ∗ WP e @ s; ⊤ {{ v, ⌜φ v⌝ }})%I) →
+       stateI σ κs ∗ WP e @ (s,0); ⊤ {{ v, ⌜φ v⌝ }})%I) →
   adequate s e σ (λ v _, φ v).
 Proof.
-  intros Hwp. apply adequate_alt; intros t2 σ2 [n [κs ?]]%erased_steps_nsteps.
-  eapply (wp_strong_adequacy Σ _); [|done]=> ?.
+  intros Hwp. apply adequate_alt; intros t2 σ2 [n [κs Hsteps]]%erased_steps_nsteps.
+  eapply (wp_strong_adequacy Σ _); [|exact Hsteps]=> ?.
   iMod Hwp as (stateI fork_post) "[Hσ Hwp]".
   iExists s, (λ σ κs _, stateI σ κs), (λ v, ⌜φ v⌝%I), fork_post.
   iIntros "{$Hσ $Hwp} !>" (e2 t2' -> ?) "_ H _".
@@ -215,16 +230,16 @@ Qed.
 Corollary wp_invariance Σ Λ `{!invPreG Σ} s e1 σ1 t2 σ2 φ :
   (∀ `{Hinv : !invG Σ} κs,
      (|={⊤}=> ∃
-         (stateI : state Λ → list (observation Λ) → nat → iProp Σ)
+         (stateI : state Λ → list (observation Λ) → list (expr Λ) → iProp Σ)
          (fork_post : val Λ → iProp Σ),
        let _ : irisG Λ Σ := IrisG _ _ Hinv stateI fork_post in
-       stateI σ1 κs 0 ∗ WP e1 @ s; ⊤ {{ _, True }} ∗
-       (stateI σ2 [] (pred (length t2)) -∗ ∃ E, |={⊤,E}=> ⌜φ⌝))%I) →
+       stateI σ1 κs [e1] ∗ WP e1 @ (s,0); ⊤ {{ _, True }} ∗
+       (stateI σ2 [] t2 -∗ ∃ E, |={⊤,E}=> ⌜φ⌝))%I) →
   rtc erased_step ([e1], σ1) (t2, σ2) →
   φ.
 Proof.
-  intros Hwp [n [κs ?]]%erased_steps_nsteps.
-  eapply (wp_strong_adequacy Σ _); [|done]=> ?.
+  intros Hwp [n [κs Hsteps]]%erased_steps_nsteps.
+  eapply (wp_strong_adequacy Σ _); [|exact Hsteps]=> ?.
   iMod (Hwp _ κs) as (stateI fork_post) "(Hσ & Hwp & Hφ)".
   iExists s, stateI, (λ _, True)%I, fork_post.
   iIntros "{$Hσ $Hwp} !>" (e2 t2' -> _) "Hσ _ _ /=".
