theories/program_logic/weakestpre.v
@@ -1,13 +1,15 @@
 From iris.proofmode Require Import base tactics classes.
 From iris.base_logic.lib Require Export fancy_updates.
 From diris.program_logic Require Export language.
+From diris.program_logic Require Export ectx_language.
+
 (* FIXME: If we import iris.bi.weakestpre earlier texan triples do not
    get pretty-printed correctly. *)
 From diris.bi Require Export weakestpre.
 Set Default Proof Using "Type".
 Import uPred.
 
-Class irisG (Λ : language) (Σ : gFunctors) := IrisG {
+Class irisG (Λ : ectxLanguage) (Σ : gFunctors) := IrisG {
   iris_invG :> invG Σ;
 
   (** The state interpretation is an invariant that should hold in between each
@@ -15,7 +17,7 @@ Class irisG (Λ : language) (Σ : gFunctors) := IrisG {
   the remaining observations, and [nat] is the number of forked-off threads
   (not the total number of threads, which is one higher because there is always
   a main thread). *) 
-  state_interp : state Λ → list (observation Λ) → nat → iProp Σ;
+  state_interp : state Λ → list (observation Λ) → list (expr Λ) → iProp Σ;
 
   (** A fixed postcondition for any forked-off thread. For most languages, e.g.
   heap_lang, this will simply be [True]. However, it is useful if one wants to
@@ -24,30 +26,32 @@ Class irisG (Λ : language) (Σ : gFunctors) := IrisG {
 }.
 Global Opaque iris_invG.
 
+
 Definition wp_pre `{!irisG Λ Σ} (s : stuckness)
-    (wp : coPset -d> expr Λ -d> (val Λ -d> iPropO Σ) -d> iPropO Σ) :
-    coPset -d> expr Λ -d> (val Λ -d> iPropO Σ) -d> iPropO Σ := λ E e1 Φ,
+    (wp : nat -d> coPset -d> expr Λ -d> (val Λ -d> iPropO Σ) -d> iPropO Σ) :
+    nat -d> coPset -d> expr Λ -d> (val Λ -d> iPropO Σ) -d> iPropO Σ := λ tid E e1 Φ,
   match to_val e1 with
   | Some v => |={E}=> Φ v
-  | None => ∀ σ1 κ κs n,
-     state_interp σ1 (κ ++ κs) n ={E,∅}=∗
+  | None => ∀ σ1 κ κs es K,
+     ⌜ es !! tid = Some (fill K e1) ⌝ -∗
+     state_interp σ1 (κ ++ κs) es ={E,∅}=∗
        ⌜if s is NotStuck then reducible e1 σ1 ∨ waiting e1 σ1 else True⌝ ∗
        ∀ e2 σ2 efs, ⌜prim_step e1 σ1 κ e2 σ2 efs⌝ ={∅,∅,E}▷=∗
-         state_interp σ2 κs (length efs + n) ∗
-         wp E e2 Φ ∗
-         [∗ list] i ↦ ef ∈ efs, wp ⊤ ef fork_post
+         state_interp σ2 κs ((<[tid := fill K e2]> es) ++ efs) ∗
+         wp tid E e2 Φ ∗
+         [∗ list] i ↦ ef ∈ efs, wp (length es + i) ⊤ ef fork_post
   end%I.
 
 Local Instance wp_pre_contractive `{!irisG Λ Σ} s : Contractive (wp_pre s).
 Proof.
-  rewrite /wp_pre=> n wp wp' Hwp E e1 Φ.
+  rewrite /wp_pre=> n wp wp' Hwp tid E e1 Φ.
   repeat (f_contractive || f_equiv); apply Hwp.
 Qed.
 
-Definition wp_def `{!irisG Λ Σ} (s : stuckness) :
-  coPset → expr Λ → (val Λ → iProp Σ) → iProp Σ := fixpoint (wp_pre s).
+Definition wp_def `{!irisG Λ Σ} (si : stuckness * nat) :
+  coPset → expr Λ → (val Λ → iProp Σ) → iProp Σ := fixpoint (wp_pre si.1) si.2.
 Definition wp_aux `{!irisG Λ Σ} : seal (@wp_def Λ Σ _). by eexists. Qed.
-Instance wp' `{!irisG Λ Σ} : Wp Λ (iProp Σ) stuckness := wp_aux.(unseal).
+Instance wp' `{!irisG Λ Σ} : Wp Λ (iProp Σ) (stuckness * nat) := wp_aux.(unseal).
 Definition wp_eq `{!irisG Λ Σ} : wp = @wp_def Λ Σ _ := wp_aux.(seal_eq).
 
 Section wp.
@@ -59,49 +63,52 @@ Implicit Types v : val Λ.
 Implicit Types e : expr Λ.
 
 (* Weakest pre *)
-Lemma wp_unfold s E e Φ :
-  WP e @ s; E {{ Φ }} ⊣⊢ wp_pre s (wp (PROP:=iProp Σ)  s) E e Φ.
-Proof. rewrite wp_eq. apply (fixpoint_unfold (wp_pre s)). Qed.
+Lemma wp_unfold s i E e Φ :
+  WP e @ (s,i); E {{ Φ }} ⊣⊢ wp_pre s (fun k => wp (PROP:=iProp Σ)  (s,k)) i E e Φ.
+Proof. rewrite wp_eq. unfold wp_def. simpl. 
+  rewrite (_ : (λ k : nat, fixpoint (wp_pre s) k) = fixpoint (wp_pre s)); last done.
+  apply (fixpoint_unfold (wp_pre s)).
+Qed.
 
-Global Instance wp_ne s E e n :
-  Proper (pointwise_relation _ (dist n) ==> dist n) (wp (PROP:=iProp Σ) s E e).
+Global Instance wp_ne s i E e n :
+  Proper (pointwise_relation _ (dist n) ==> dist n) (wp (PROP:=iProp Σ) (s,i) E e).
 Proof.
   revert e. induction (lt_wf n) as [n _ IH]=> e Φ Ψ HΦ.
   rewrite !wp_unfold /wp_pre.
   (* FIXME: figure out a way to properly automate this proof *)
   (* FIXME: reflexivity, as being called many times by f_equiv and f_contractive
   is very slow here *)
-  do 24 (f_contractive || f_equiv). apply IH; first lia.
+  do 27 (f_contractive || f_equiv). apply IH; first lia.
   intros v. eapply dist_le; eauto with lia.
 Qed.
-Global Instance wp_proper s E e :
-  Proper (pointwise_relation _ (≡) ==> (≡)) (wp (PROP:=iProp Σ) s E e).
+Global Instance wp_proper s i E e :
+  Proper (pointwise_relation _ (≡) ==> (≡)) (wp (PROP:=iProp Σ) (s,i) E e).
 Proof.
   by intros Φ Φ' ?; apply equiv_dist=>n; apply wp_ne=>v; apply equiv_dist.
 Qed.
-Global Instance wp_contractive s E e n :
+Global Instance wp_contractive s i E e n :
   TCEq (to_val e) None →
-  Proper (pointwise_relation _ (dist_later n) ==> dist n) (wp (PROP:=iProp Σ) s E e).
+  Proper (pointwise_relation _ (dist_later n) ==> dist n) (wp (PROP:=iProp Σ) (s,i) E e).
 Proof.
   intros He Φ Ψ HΦ. rewrite !wp_unfold /wp_pre He.
   by repeat (f_contractive || f_equiv).
 Qed.
 
-Lemma wp_value' s E Φ v : Φ v ⊢ WP of_val v @ s; E {{ Φ }}.
+Lemma wp_value' s i E Φ v : Φ v ⊢ WP of_val v @ (s,i); E {{ Φ }}.
 Proof. iIntros "HΦ". rewrite wp_unfold /wp_pre to_of_val. auto. Qed.
-Lemma wp_value_inv' s E Φ v : WP of_val v @ s; E {{ Φ }} ={E}=∗ Φ v.
+Lemma wp_value_inv' s i E Φ v : WP of_val v @ (s,i); E {{ Φ }} ={E}=∗ Φ v.
 Proof. by rewrite wp_unfold /wp_pre to_of_val. Qed.
 
-Lemma wp_strong_mono s1 s2 E1 E2 e Φ Ψ :
+Lemma wp_strong_mono s1 s2 i E1 E2 e Φ Ψ :
   s1 ⊑ s2 → E1 ⊆ E2 →
-  WP e @ s1; E1 {{ Φ }} -∗ (∀ v, Φ v ={E2}=∗ Ψ v) -∗ WP e @ s2; E2 {{ Ψ }}.
+  WP e @ (s1,i); E1 {{ Φ }} -∗ (∀ v, Φ v ={E2}=∗ Ψ v) -∗ WP e @ (s2,i); E2 {{ Ψ }}.
 Proof.
-  iIntros (? HE) "H HΦ". iLöb as "IH" forall (e E1 E2 HE Φ Ψ).
+  iIntros (? HE) "H HΦ". iLöb as "IH" forall (e i E1 E2 HE Φ Ψ).
   rewrite !wp_unfold /wp_pre.
   destruct (to_val e) as [v|] eqn:?.
   { iApply ("HΦ" with "[> -]"). by iApply (fupd_mask_mono E1 _). }
-  iIntros (σ1 κ κs n) "Hσ". iMod (fupd_intro_mask' E2 E1) as "Hclose"; first done.
-  iMod ("H" with "[$]") as "[% H]".
+  iIntros (σ1 κ κs es K ?) "Hσ". iMod (fupd_intro_mask' E2 E1) as "Hclose"; first done.
+  iMod ("H" with "[//] [$]") as "[% H]".
   iModIntro. iSplit; [by destruct s1, s2|]. iIntros (e2 σ2 efs Hstep).
   iMod ("H" with "[//]") as "H". iIntros "!> !>".
   iMod "H" as "(Hσ & H & Hefs)".
@@ -111,28 +118,30 @@ Proof.
     iIntros "H". iApply ("IH" with "[] H"); auto.
 Qed.
 
-Lemma fupd_wp s E e Φ : (|={E}=> WP e @ s; E {{ Φ }}) ⊢ WP e @ s; E {{ Φ }}.
+Lemma fupd_wp s i E e Φ : (|={E}=> WP e @ (s,i); E {{ Φ }}) ⊢ WP e @ (s,i); E {{ Φ }}.
 Proof.
   rewrite wp_unfold /wp_pre. iIntros "H". destruct (to_val e) as [v|] eqn:?.
   { by iMod "H". }
-  iIntros (σ1 κ κs n) "Hσ1". iMod "H". by iApply "H".
+  iIntros (σ1 κ κs es K ?) "Hσ1". iMod "H". by iApply "H".
 Qed.
-Lemma wp_fupd s E e Φ : WP e @ s; E {{ v, |={E}=> Φ v }} ⊢ WP e @ s; E {{ Φ }}.
-Proof. iIntros "H". iApply (wp_strong_mono s s E with "H"); auto. Qed.
+Lemma wp_fupd s i E e Φ : WP e @ (s,i); E {{ v, |={E}=> Φ v }} ⊢ WP e @ (s,i); E {{ Φ }}.
+Proof. iIntros "H". iApply (wp_strong_mono s s i E with "H"); auto. Qed.
 
-Lemma wp_atomic s E1 E2 e Φ `{!Atomic (stuckness_to_atomicity s) e} :
-  (|={E1,E2}=> WP e @ s; E2 {{ v, |={E2,E1}=> Φ v }}) ⊢ WP e @ s; E1 {{ Φ }}.
+Lemma wp_atomic s i E1 E2 e Φ `{!Atomic (stuckness_to_atomicity s) e} :
+  (|={E1,E2}=> WP e @ (s,i); E2 {{ v, |={E2,E1}=> Φ v }}) ⊢ WP e @ (s,i); E1 {{ Φ }}.
 Proof.
   iIntros "H". rewrite !wp_unfold /wp_pre.
   destruct (to_val e) as [v|] eqn:He.
   { by iDestruct "H" as ">>> $". }
-  iIntros (σ1 κ κs n) "Hσ". iMod "H". iMod ("H" $! σ1 with "Hσ") as "[$ H]".
+  iIntros (σ1 κ κs es K ?) "Hσ". iMod "H". iMod ("H" $! σ1 with "[//] Hσ") as "[$ H]".
   iModIntro. iIntros (e2 σ2 efs Hstep).
   iMod ("H" with "[//]") as "H". iIntros "!>!>".
   iMod "H" as "(Hσ & H & Hefs)". destruct s.
   - rewrite !wp_unfold /wp_pre. destruct (to_val e2) as [v2|] eqn:He2.
     + iDestruct "H" as ">> $". by iFrame.
-    + iMod ("H" $! _ [] with "[$]") as "[H _]". iDestruct "H" as %[H|H]. 
+    + iMod ("H" $! _ [] with "[%] [$]") as "[H _]". 
+      { apply lookup_app_l_Some. apply list_lookup_insert. by eapply lookup_lt_Some. }
+      iDestruct "H" as %[H|H]. 
       * destruct H as (? & ? & ? & ? & ?). apply atomic in Hstep as [? ?].
         edestruct H0. eauto.
       * apply atomic in Hstep as [? ?]. done.
@@ -141,39 +150,40 @@ Proof.
     iModIntro. iFrame "Hσ Hefs". by iApply wp_value'.
 Qed.
 
-Lemma wp_step_fupd s E1 E2 e P Φ :
+Lemma wp_step_fupd s i E1 E2 e P Φ :
   to_val e = None → E2 ⊆ E1 →
-  (|={E1,E2}▷=> P) -∗ WP e @ s; E2 {{ v, P ={E1}=∗ Φ v }} -∗ WP e @ s; E1 {{ Φ }}.
+  (|={E1,E2}▷=> P) -∗ WP e @ (s,i); E2 {{ v, P ={E1}=∗ Φ v }} -∗ WP e @ (s,i); E1 {{ Φ }}.
 Proof.
   rewrite !wp_unfold /wp_pre. iIntros (-> ?) "HR H".
-  iIntros (σ1 κ κs n) "Hσ". iMod "HR". iMod ("H" with "[$]") as "[$ H]".
+  iIntros (σ1 κ κs es K ?) "Hσ". iMod "HR". iMod ("H" with "[//] [$]") as "[$ H]".
   iIntros "!>" (e2 σ2 efs Hstep). iMod ("H" $! e2 σ2 efs with "[% //]") as "H".
   iIntros "!>!>". iMod "H" as "(Hσ & H & Hefs)".
   iMod "HR". iModIntro. iFrame "Hσ Hefs".
-  iApply (wp_strong_mono s s E2 with "H"); [done..|].
+  iApply (wp_strong_mono s s i E2 with "H"); [done..|].
   iIntros (v) "H". by iApply "H".
 Qed.
 
-Lemma wp_bind K `{!LanguageCtx K} s E e Φ :
-  WP e @ s; E {{ v, WP K (of_val v) @ s; E {{ Φ }} }} ⊢ WP K e @ s; E {{ Φ }}.
+Lemma wp_bind K s i E e Φ :
+  WP e @ (s,i); E {{ v, WP fill K (of_val v) @ (s,i); E {{ Φ }} }} ⊢ WP fill K e @ (s,i); E {{ Φ }}.
 Proof.
-  iIntros "H". iLöb as "IH" forall (E e Φ). rewrite wp_unfold /wp_pre.
+  iIntros "H". iLöb as "IH" forall (E e i Φ). rewrite wp_unfold /wp_pre.
   destruct (to_val e) as [v|] eqn:He.
   { apply of_to_val in He as <-. by iApply fupd_wp. }
   rewrite wp_unfold /wp_pre fill_not_val //.
-  iIntros (σ1 κ κs n) "Hσ". iMod ("H" with "[$]") as "[% H]". iModIntro; iSplit.
-  { iPureIntro. destruct s; last done.
-    unfold reducible in *. destruct H.
-    - naive_solver eauto using fill_step.
-    - right. destruct LanguageCtx0. eauto. }
+  iIntros (σ1 κ κs es K' ?) "Hσ". rewrite fill_comp in a. iMod ("H" with "[//] [$]") as "[% H]".
+  iModIntro; iSplit.
+  { iPureIntro. destruct s; last done. destruct H.
+    - left. eauto using fill_reducible.
+    - right. apply waiting_fill. exact H. }
   iIntros (e2 σ2 efs Hstep).
-  destruct (fill_step_inv e σ1 κ e2 σ2 efs) as (e2'&->&?); auto.
+  destruct (fill_step_inv e σ1 κ e2 σ2 efs) as (e2'&->&?); [done..|].
   iMod ("H" $! e2' σ2 efs with "[//]") as "H". iIntros "!>!>".
   iMod "H" as "(Hσ & H & Hefs)".
-  iModIntro. iFrame "Hσ Hefs". by iApply "IH".
+  iModIntro. rewrite fill_comp. iFrame "Hσ Hefs". by iApply "IH".
 Qed.
 
-Lemma wp_bind_inv K `{!LanguageCtx K} s E e Φ :
+(* No longer holds!  *)
+(* Lemma wp_bind_inv K `{!LanguageCtx K} s E e Φ :
   WP K e @ s; E {{ Φ }} ⊢ WP e @ s; E {{ v, WP K (of_val v) @ s; E {{ Φ }} }}.
 Proof.
   iIntros "H". iLöb as "IH" forall (E e Φ). rewrite !wp_unfold /wp_pre.
@@ -186,79 +196,81 @@ Proof.
   iMod ("H" $! (K e2) σ2 efs with "[]") as "H"; [by eauto using fill_step|].
   iIntros "!>!>". iMod "H" as "(Hσ & H & Hefs)".
   iModIntro. iFrame "Hσ Hefs". by iApply "IH".
-Qed.
+Qed. *)
 
 (** * Derived rules *)
-Lemma wp_mono s E e Φ Ψ : (∀ v, Φ v ⊢ Ψ v) → WP e @ s; E {{ Φ }} ⊢ WP e @ s; E {{ Ψ }}.
+Lemma wp_mono s i E e Φ Ψ : (∀ v, Φ v ⊢ Ψ v) → WP e @ (s,i); E {{ Φ }} ⊢ WP e @ (s,i); E {{ Ψ }}.
 Proof.
   iIntros (HΦ) "H"; iApply (wp_strong_mono with "H"); auto.
   iIntros (v) "?". by iApply HΦ.
 Qed.
-Lemma wp_stuck_mono s1 s2 E e Φ :
-  s1 ⊑ s2 → WP e @ s1; E {{ Φ }} ⊢ WP e @ s2; E {{ Φ }}.
+Lemma wp_stuck_mono s1 s2 i E e Φ :
+  s1 ⊑ s2 → WP e @ (s1,i); E {{ Φ }} ⊢ WP e @ (s2,i); E {{ Φ }}.
 Proof. iIntros (?) "H". iApply (wp_strong_mono with "H"); auto. Qed.
-Lemma wp_stuck_weaken s E e Φ :
-  WP e @ s; E {{ Φ }} ⊢ WP e @ E ?{{ Φ }}.
+
+(* Jules TODO *)
+Lemma wp_stuck_weaken s i E e Φ :
+  WP e @ (s,i); E {{ Φ }} ⊢ WP e @ (MaybeStuck,i); E {{ Φ }}.
 Proof. apply wp_stuck_mono. by destruct s. Qed.
-Lemma wp_mask_mono s E1 E2 e Φ : E1 ⊆ E2 → WP e @ s; E1 {{ Φ }} ⊢ WP e @ s; E2 {{ Φ }}.
+Lemma wp_mask_mono s i E1 E2 e Φ : E1 ⊆ E2 → WP e @ (s,i); E1 {{ Φ }} ⊢ WP e @ (s,i); E2 {{ Φ }}.
 Proof. iIntros (?) "H"; iApply (wp_strong_mono with "H"); auto. Qed.
-Global Instance wp_mono' s E e :
-  Proper (pointwise_relation _ (⊢) ==> (⊢)) (wp (PROP:=iProp Σ) s E e).
+Global Instance wp_mono' s i E e :
+  Proper (pointwise_relation _ (⊢) ==> (⊢)) (wp (PROP:=iProp Σ) (s,i) E e).
 Proof. by intros Φ Φ' ?; apply wp_mono. Qed.
-Global Instance wp_flip_mono' s E e :
-  Proper (pointwise_relation _ (flip (⊢)) ==> (flip (⊢))) (wp (PROP:=iProp Σ) s E e).
+Global Instance wp_flip_mono' s i E e :
+  Proper (pointwise_relation _ (flip (⊢)) ==> (flip (⊢))) (wp (PROP:=iProp Σ) (s,i) E e).
 Proof. by intros Φ Φ' ?; apply wp_mono. Qed.
 
-Lemma wp_value s E Φ e v : IntoVal e v → Φ v ⊢ WP e @ s; E {{ Φ }}.
+Lemma wp_value s i E Φ e v : IntoVal e v → Φ v ⊢ WP e @ (s,i); E {{ Φ }}.
 Proof. intros <-. by apply wp_value'. Qed.
-Lemma wp_value_fupd' s E Φ v : (|={E}=> Φ v) ⊢ WP of_val v @ s; E {{ Φ }}.
+Lemma wp_value_fupd' s i E Φ v : (|={E}=> Φ v) ⊢ WP of_val v @ (s,i); E {{ Φ }}.
 Proof. intros. by rewrite -wp_fupd -wp_value'. Qed.
-Lemma wp_value_fupd s E Φ e v `{!IntoVal e v} :
-  (|={E}=> Φ v) ⊢ WP e @ s; E {{ Φ }}.
+Lemma wp_value_fupd s i E Φ e v `{!IntoVal e v} :
+  (|={E}=> Φ v) ⊢ WP e @ (s,i); E {{ Φ }}.
 Proof. intros. rewrite -wp_fupd -wp_value //. Qed.
-Lemma wp_value_inv s E Φ e v : IntoVal e v → WP e @ s; E {{ Φ }} ={E}=∗ Φ v.
+Lemma wp_value_inv s i E Φ e v : IntoVal e v → WP e @ (s,i); E {{ Φ }} ={E}=∗ Φ v.
 Proof. intros <-. by apply wp_value_inv'. Qed.
 
-Lemma wp_frame_l s E e Φ R : R ∗ WP e @ s; E {{ Φ }} ⊢ WP e @ s; E {{ v, R ∗ Φ v }}.
+Lemma wp_frame_l s i E e Φ R : R ∗ WP e @ (s,i); E {{ Φ }} ⊢ WP e @ (s,i); E {{ v, R ∗ Φ v }}.
 Proof. iIntros "[? H]". iApply (wp_strong_mono with "H"); auto with iFrame. Qed.
-Lemma wp_frame_r s E e Φ R : WP e @ s; E {{ Φ }} ∗ R ⊢ WP e @ s; E {{ v, Φ v ∗ R }}.
+Lemma wp_frame_r s i E e Φ R : WP e @ (s,i); E {{ Φ }} ∗ R ⊢ WP e @ (s,i); E {{ v, Φ v ∗ R }}.
 Proof. iIntros "[H ?]". iApply (wp_strong_mono with "H"); auto with iFrame. Qed.
 
-Lemma wp_frame_step_l s E1 E2 e Φ R :
+Lemma wp_frame_step_l s i E1 E2 e Φ R :
   to_val e = None → E2 ⊆ E1 →
-  (|={E1,E2}▷=> R) ∗ WP e @ s; E2 {{ Φ }} ⊢ WP e @ s; E1 {{ v, R ∗ Φ v }}.
+  (|={E1,E2}▷=> R) ∗ WP e @ (s,i); E2 {{ Φ }} ⊢ WP e @ (s,i); E1 {{ v, R ∗ Φ v }}.
 Proof.
   iIntros (??) "[Hu Hwp]". iApply (wp_step_fupd with "Hu"); try done.
   iApply (wp_mono with "Hwp"). by iIntros (?) "$$".
 Qed.
-Lemma wp_frame_step_r s E1 E2 e Φ R :
+Lemma wp_frame_step_r s i E1 E2 e Φ R :
   to_val e = None → E2 ⊆ E1 →
-  WP e @ s; E2 {{ Φ }} ∗ (|={E1,E2}▷=> R) ⊢ WP e @ s; E1 {{ v, Φ v ∗ R }}.
+  WP e @ (s,i); E2 {{ Φ }} ∗ (|={E1,E2}▷=> R) ⊢ WP e @ (s,i); E1 {{ v, Φ v ∗ R }}.
 Proof.
   rewrite [(WP _ @ _; _ {{ _ }} ∗ _)%I]comm; setoid_rewrite (comm _ _ R).
   apply wp_frame_step_l.
 Qed.
-Lemma wp_frame_step_l' s E e Φ R :
-  to_val e = None → ▷ R ∗ WP e @ s; E {{ Φ }} ⊢ WP e @ s; E {{ v, R ∗ Φ v }}.
-Proof. iIntros (?) "[??]". iApply (wp_frame_step_l s E E); try iFrame; eauto. Qed.
-Lemma wp_frame_step_r' s E e Φ R :
-  to_val e = None → WP e @ s; E {{ Φ }} ∗ ▷ R ⊢ WP e @ s; E {{ v, Φ v ∗ R }}.
-Proof. iIntros (?) "[??]". iApply (wp_frame_step_r s E E); try iFrame; eauto. Qed.
+Lemma wp_frame_step_l' s i E e Φ R :
+  to_val e = None → ▷ R ∗ WP e @ (s,i); E {{ Φ }} ⊢ WP e @ (s,i); E {{ v, R ∗ Φ v }}.
+Proof. iIntros (?) "[??]". iApply (wp_frame_step_l s i E E); try iFrame; eauto. Qed.
+Lemma wp_frame_step_r' s i E e Φ R :
+  to_val e = None → WP e @ (s,i); E {{ Φ }} ∗ ▷ R ⊢ WP e @ (s,i); E {{ v, Φ v ∗ R }}.
+Proof. iIntros (?) "[??]". iApply (wp_frame_step_r s i E E); try iFrame; eauto. Qed.
 
-Lemma wp_wand s E e Φ Ψ :
-  WP e @ s; E {{ Φ }} -∗ (∀ v, Φ v -∗ Ψ v) -∗ WP e @ s; E {{ Ψ }}.
+Lemma wp_wand s i E e Φ Ψ :
+  WP e @ (s,i); E {{ Φ }} -∗ (∀ v, Φ v -∗ Ψ v) -∗ WP e @ (s,i); E {{ Ψ }}.
 Proof.
   iIntros "Hwp H". iApply (wp_strong_mono with "Hwp"); auto.
   iIntros (?) "?". by iApply "H".
 Qed.
-Lemma wp_wand_l s E e Φ Ψ :
-  (∀ v, Φ v -∗ Ψ v) ∗ WP e @ s; E {{ Φ }} ⊢ WP e @ s; E {{ Ψ }}.
+Lemma wp_wand_l s i E e Φ Ψ :
+  (∀ v, Φ v -∗ Ψ v) ∗ WP e @ (s,i); E {{ Φ }} ⊢ WP e @ (s,i); E {{ Ψ }}.
 Proof. iIntros "[H Hwp]". iApply (wp_wand with "Hwp H"). Qed.
-Lemma wp_wand_r s E e Φ Ψ :
-  WP e @ s; E {{ Φ }} ∗ (∀ v, Φ v -∗ Ψ v) ⊢ WP e @ s; E {{ Ψ }}.
+Lemma wp_wand_r s i E e Φ Ψ :
+  WP e @ (s,i); E {{ Φ }} ∗ (∀ v, Φ v -∗ Ψ v) ⊢ WP e @ (s,i); E {{ Ψ }}.
 Proof. iIntros "[Hwp H]". iApply (wp_wand with "Hwp H"). Qed.
-Lemma wp_frame_wand_l s E e Q Φ :
-  Q ∗ WP e @ s; E {{ v, Q -∗ Φ v }} -∗ WP e @ s; E {{ Φ }}.
+Lemma wp_frame_wand_l s i E e Q Φ :
+  Q ∗ WP e @ (s,i); E {{ v, Q -∗ Φ v }} -∗ WP e @ (s,i); E {{ Φ }}.
 Proof.
   iIntros "[HQ HWP]". iApply (wp_wand with "HWP").
   iIntros (v) "HΦ". by iApply "HΦ".
@@ -272,46 +284,46 @@ Section proofmode_classes.
   Implicit Types P Q : iProp Σ.
   Implicit Types Φ : val Λ → iProp Σ.
 
-  Global Instance frame_wp p s E e R Φ Ψ :
+  Global Instance frame_wp p s i E e R Φ Ψ :
     (∀ v, Frame p R (Φ v) (Ψ v)) →
-    Frame p R (WP e @ s; E {{ Φ }}) (WP e @ s; E {{ Ψ }}).
+    Frame p R (WP e @ (s,i); E {{ Φ }}) (WP e @ (s,i); E {{ Ψ }}).
   Proof. rewrite /Frame=> HR. rewrite wp_frame_l. apply wp_mono, HR. Qed.
 
-  Global Instance is_except_0_wp s E e Φ : IsExcept0 (WP e @ s; E {{ Φ }}).
+  Global Instance is_except_0_wp s i E e Φ : IsExcept0 (WP e @ (s,i); E {{ Φ }}).
   Proof. by rewrite /IsExcept0 -{2}fupd_wp -except_0_fupd -fupd_intro. Qed.
 
-  Global Instance elim_modal_bupd_wp p s E e P Φ :
-    ElimModal True p false (|==> P) P (WP e @ s; E {{ Φ }}) (WP e @ s; E {{ Φ }}).
+  Global Instance elim_modal_bupd_wp p s i E e P Φ :
+    ElimModal True p false (|==> P) P (WP e @ (s,i); E {{ Φ }}) (WP e @ (s,i); E {{ Φ }}).
   Proof.
     by rewrite /ElimModal intuitionistically_if_elim
       (bupd_fupd E) fupd_frame_r wand_elim_r fupd_wp.
   Qed.
 
-  Global Instance elim_modal_fupd_wp p s E e P Φ :
-    ElimModal True p false (|={E}=> P) P (WP e @ s; E {{ Φ }}) (WP e @ s; E {{ Φ }}).
+  Global Instance elim_modal_fupd_wp p s i E e P Φ :
+    ElimModal True p false (|={E}=> P) P (WP e @ (s,i); E {{ Φ }}) (WP e @ (s,i); E {{ Φ }}).
   Proof.
     by rewrite /ElimModal intuitionistically_if_elim
       fupd_frame_r wand_elim_r fupd_wp.
   Qed.
 
-  Global Instance elim_modal_fupd_wp_atomic p s E1 E2 e P Φ :
+  Global Instance elim_modal_fupd_wp_atomic p s i E1 E2 e P Φ :
     Atomic (stuckness_to_atomicity s) e →
     ElimModal True p false (|={E1,E2}=> P) P
-            (WP e @ s; E1 {{ Φ }}) (WP e @ s; E2 {{ v, |={E2,E1}=> Φ v }})%I.
+            (WP e @ (s,i); E1 {{ Φ }}) (WP e @ (s,i); E2 {{ v, |={E2,E1}=> Φ v }})%I.
   Proof.
     intros. by rewrite /ElimModal intuitionistically_if_elim
       fupd_frame_r wand_elim_r wp_atomic.
   Qed.
 
-  Global Instance add_modal_fupd_wp s E e P Φ :
-    AddModal (|={E}=> P) P (WP e @ s; E {{ Φ }}).
+  Global Instance add_modal_fupd_wp s i E e P Φ :
+    AddModal (|={E}=> P) P (WP e @ (s,i); E {{ Φ }}).
   Proof. by rewrite /AddModal fupd_frame_r wand_elim_r fupd_wp. Qed.
 
-  Global Instance elim_acc_wp {X} E1 E2 α β γ e s Φ :
+  Global Instance elim_acc_wp {X} E1 E2 α β γ e s i Φ :
     Atomic (stuckness_to_atomicity s) e →
     ElimAcc (X:=X) (fupd E1 E2) (fupd E2 E1)
-            α β γ (WP e @ s; E1 {{ Φ }})
-            (λ x, WP e @ s; E2 {{ v, |={E2}=> β x ∗ (γ x -∗? Φ v) }})%I.
+            α β γ (WP e @ (s,i); E1 {{ Φ }})
+            (λ x, WP e @ (s,i); E2 {{ v, |={E2}=> β x ∗ (γ x -∗? Φ v) }})%I.
   Proof.
     intros ?. rewrite /ElimAcc.
     iIntros "Hinner >Hacc". iDestruct "Hacc" as (x) "[Hα Hclose]".
@@ -319,10 +331,10 @@ Section proofmode_classes.
     iIntros (v) ">[Hβ HΦ]". iApply "HΦ". by iApply "Hclose".
   Qed.
 
-  Global Instance elim_acc_wp_nonatomic {X} E α β γ e s Φ :
+  Global Instance elim_acc_wp_nonatomic {X} E α β γ e s i Φ :
     ElimAcc (X:=X) (fupd E E) (fupd E E)
-            α β γ (WP e @ s; E {{ Φ }})
-            (λ x, WP e @ s; E {{ v, |={E}=> β x ∗ (γ x -∗? Φ v) }})%I.
+            α β γ (WP e @ (s,i); E {{ Φ }})
+            (λ x, WP e @ (s,i); E {{ v, |={E}=> β x ∗ (γ x -∗? Φ v) }})%I.
   Proof.
     rewrite /ElimAcc.
     iIntros "Hinner >Hacc". iDestruct "Hacc" as (x) "[Hα Hclose]".
