theories/test.v
@@ -1,3 +1,136 @@
+From iris.proofmode Require Import tactics.
+
+Fixpoint evalp (x : Z) (p : list Z) : Z :=
+  match p with
+  | [] => 0
+  | a :: p' => a * x ^ (length p') + evalp x p'
+  end%Z.
+
+Fixpoint zero (p : list Z) :=
+  match p with
+  | [] => True
+  | a :: p' => a = 0 /\ zero p'
+  end.
+
+
+Lemma zero_if_ext_zero p :
+  (forall n, evalp n p = 0) -> zero p.
+Proof.
+  induction p; first done. simpl.
+  intros. assert (a=0); last (subst;auto). clear IHp.
+  
+Qed.
+
+Lemma zero_if_ext_zero' (p : list nat) :
+  (forall n, evalp n p = 0) -> (forall i a, p !! i = Some a -> a=0).
+Proof.
+  intros. specialize (H 1).
+  induction p; first done.
+  intros.
+  intros. assert (a=0);[|subst;simpl;auto].
+  specialize (H 1). simpl in H. rewrite Nat.pow_1_l in H. lia.
+Qed.
+
+Lemma foo (P : nat -> Prop) :
+  (forall n, (forall m, m < n -> P m) -> P n) -> (forall n m, m < n -> P m).
+Proof.
+    intros H n. induction n.
+    - lia.
+    - intros. apply H. intros. apply IHn. lia.
+Qed.
+
+Lemma bar (P : nat -> Prop) :
+  (forall n, (forall m, m < n -> P m) -> P n) -> (forall n, P n).
+Proof.
+  intros. apply H. induction n.
+  - lia.
+  - intros. apply H. intros. apply IHn. lia.
+Qed.
+
+Ltac doind :=
+  match goal with
+  | x : _ |- _ => induction x; simpl
+  end.
+
+Hint Extern 200 => doind : induction.
+
+Lemma foo' (P : nat -> Prop) :
+  (forall n, (forall m, m < n -> P m) -> P n) -> (forall n, P n).
+Proof.
+    eauto with induction lia.
+Qed.
+
+Ltac dorew :=
+  match goal with
+  | x : _ |- _ => rewrite x || rewrite<- x
+  end.
+
+Hint Extern 100 => dorew : rewrite.
+
+Inductive N : Type := Z : N | S : N -> N.
+
+Fixpoint plus a b :=
+  match a with
+  | Z => b
+  | S a' => S (plus a' b)
+  end.
+
+Lemma plus_comm : forall a b, plus a b = plus b a.
+Proof.
+  eauto 7 with induction rewrite.
+Qed.
+
+Lemma plus_assoc : forall a b c, plus (plus a b) c = plus a (plus b c).
+Proof.
+  eauto with induction rewrite.
+Qed.
+
+Definition t_id := forall t:Type, t -> t.
+Definition p1_id f := forall a, forall P : a -> Prop, forall x, P x -> P (f a x).
+
+Lemma all_id (f : t_id) : p1_id f -> forall a x, f a x = x.
+Proof.
+  unfold p1_id. intros. apply H. auto.
+Qed.
+
+Definition cnat := forall t:Prop, t -> (t -> t) -> t.
+
+Definition cZ : cnat := fun t z f => z.
+Definition cS (n : cnat) : cnat := fun t z f => f (n t z f).
+
+Definition p2_nat f g := 
+  forall a b, forall R : a -> b -> Prop,
+  forall x y s r, R x y -> (forall x' y', R x' y' -> R (s x') (r y')) -> R (f a x s) (g b y r).
+
+Lemma cnat_repr : (forall n:cnat, n cnat cZ cS = n).
+
+Lemma cnat_ind : (forall n:cnat, p2_nat n n) -> forall P : cnat -> Prop, P cZ -> (forall n, P n -> P (cS n)) -> forall n, P n.
+Proof.
+  unfold p2_nat.
+  intros.
+
+
+Inductive A := fooA : A.
+Inductive B := fooB : B.
+Inductive C := fooC : C.
+Inductive D := fooD : D.
+
+Class R (x : Type) (y : Type) : Type := { foo : nat }.
+
+Check R.
+
+Instance I4 {x y z : Type} (a1 : R x y) (a2 : R y z) : R x z := { foo := 4 }.
+Instance I5 (a1 : R A A) : R A D := { foo := 5 }.
+
+Instance I1 : R A B := { foo := 1 }.
+Instance I2 : R A C := { foo := 2 }.
+Instance I3 : R C D := { foo := 3 }.
+
+Definition bar `{x : R A D} := 2.
+Definition baz `{x : R A A} := 3.
+Set Typeclasses Iterative Deepening.
+Compute bar.
+
 From diris.heap_lang Require Export proofmode notation.
 Set Default Proof Using "Type".
 
