theories/program_logic/lifting.v
@@ -13,27 +13,27 @@ Implicit Types Φ : val Λ → iProp Σ.
 
 Hint Resolve reducible_no_obs_reducible : core.
 
-Lemma wp_lift_step_fupd s E Φ e1 :
+Lemma wp_lift_step_fupd s i E Φ e1 :
   to_val e1 = None →
-  (∀ σ1 κ κs n, state_interp σ1 (κ ++ κs) n ={E,∅}=∗
+  (∀ σ1 κ κs es K, state_interp σ1 (κ ++ κs) es ={E,∅}=∗
     ⌜if s is NotStuck then reducible e1 σ1 ∨ waiting e1 σ1 else True⌝ ∗
     ∀ e2 σ2 efs, ⌜prim_step e1 σ1 κ e2 σ2 efs⌝ ={∅,∅,E}▷=∗
-      state_interp σ2 κs (length efs + n) ∗
-      WP e2 @ s; E {{ Φ }} ∗
-      [∗ list] ef ∈ efs, WP ef @ s; ⊤ {{ fork_post }})
-  ⊢ WP e1 @ s; E {{ Φ }}.
+      state_interp σ2 κs ((<[i := fill K e2]> es) ++ efs) ∗
+      WP e2 @ (s,i); E {{ Φ }} ∗
+      [∗ list] i ↦ ef ∈ efs, WP ef @ (s,length es + i); ⊤ {{ fork_post }})
+  ⊢ WP e1 @ (s,i); E {{ Φ }}.
 Proof.
-  rewrite wp_unfold /wp_pre=>->. iIntros "H" (σ1 κ κs n) "Hσ".
+  rewrite wp_unfold /wp_pre=>->. iIntros "H" (σ1 κ κs es K) "Hf Hσ".
   iMod ("H" with "Hσ") as "(%&H)". iModIntro. iSplit. by destruct s.
   iIntros (????). iApply "H". eauto.
 Qed.
 
-Lemma wp_lift_stuck E Φ e :
+Lemma wp_lift_stuck E Φ e i :
   to_val e = None →
-  (∀ σ κs n, state_interp σ κs n ={E,∅}=∗ ⌜stuck e σ⌝)
-  ⊢ WP e @ E ?{{ Φ }}.
+  (∀ σ κs es, state_interp σ κs es ={E,∅}=∗ ⌜stuck e σ⌝)
+  ⊢ WP e @ (MaybeStuck,i); E {{ Φ }}.
 Proof.
-  rewrite wp_unfold /wp_pre=>->. iIntros "H" (σ1 κ κs n) "Hσ".
+  rewrite wp_unfold /wp_pre=>->. iIntros "H" (σ1 κ κs es K) "Hf Hσ".
   iMod ("H" with "Hσ") as %[? Hirr]. iModIntro. iSplit; first done.
   iIntros (e2 σ2 efs ?). 
   destruct Hirr as [Hirr H1].
@@ -41,41 +41,42 @@ Proof.
 Qed.
 
 (** Derived lifting lemmas. *)
-Lemma wp_lift_step s E Φ e1 :
+Lemma wp_lift_step s i E Φ e1 :
   to_val e1 = None →
-  (∀ σ1 κ κs n, state_interp σ1 (κ ++ κs) n ={E,∅}=∗
+  (∀ σ1 κ κs es K, state_interp σ1 (κ ++ κs) es ={E,∅}=∗
     ⌜if s is NotStuck then reducible e1 σ1 ∨ waiting e1 σ1 else True⌝ ∗
     ▷ ∀ e2 σ2 efs, ⌜prim_step e1 σ1 κ e2 σ2 efs⌝ ={∅,E}=∗
-      state_interp σ2 κs (length efs + n) ∗
-      WP e2 @ s; E {{ Φ }} ∗
-      [∗ list] ef ∈ efs, WP ef @ s; ⊤ {{ fork_post }})
-  ⊢ WP e1 @ s; E {{ Φ }}.
+      state_interp σ2 κs ((<[i := fill K e2]> es) ++ efs) ∗
+      WP e2 @ (s,i); E {{ Φ }} ∗
+      [∗ list] i ↦ ef ∈ efs, WP ef @ (s,length es + i); ⊤ {{ fork_post }})
+  ⊢ WP e1 @ (s,i); E {{ Φ }}.
 Proof.
-  iIntros (?) "H". iApply wp_lift_step_fupd; [done|]. iIntros (????) "Hσ".
+  iIntros (?) "H". iApply wp_lift_step_fupd; [done|]. iIntros (?????) "Hσ".
   iMod ("H" with "Hσ") as "[$ H]". iIntros "!> * % !> !>". by iApply "H".
 Qed.
 
-Lemma wp_lift_pure_step_no_fork `{!Inhabited (state Λ)} s E E' Φ e1 :
+Lemma wp_lift_pure_step_no_fork `{!Inhabited (state Λ)} s i E E' Φ e1 :
   (∀ σ1, if s is NotStuck then reducible e1 σ1 ∨ waiting e1 σ1 else to_val e1 = None) →
   (∀ κ σ1 e2 σ2 efs, prim_step e1 σ1 κ e2 σ2 efs → κ = [] ∧ σ2 = σ1 ∧ efs = []) →
-  (|={E,E'}▷=> ∀ κ e2 efs σ, ⌜prim_step e1 σ κ e2 σ efs⌝ → WP e2 @ s; E {{ Φ }})
-  ⊢ WP e1 @ s; E {{ Φ }}.
+  (|={E,E'}▷=> ∀ κ e2 efs σ, ⌜prim_step e1 σ κ e2 σ efs⌝ → WP e2 @ (s,i); E {{ Φ }})
+  ⊢ WP e1 @ (s,i); E {{ Φ }}.
 Proof.
   iIntros (Hsafe Hstep) "H". iApply wp_lift_step.
   { specialize (Hsafe inhabitant).
     destruct s; naive_solver eauto using reducible_not_val, waiting_not_val. }
-  iIntros (σ1 κ κs n) "Hσ". iMod "H".
+  iIntros (σ1 κ κs es K) "Hσ". iMod "H".
   iMod fupd_intro_mask' as "Hclose"; last iModIntro; first by set_solver. iSplit.
   { iPureIntro. destruct s; done. }
   iNext. iIntros (e2 σ2 efs ?).
   destruct (Hstep κ σ1 e2 σ2 efs) as (-> & <- & ->); auto.
   iMod "Hclose" as "_". iMod "H". iModIntro.
-  iDestruct ("H" with "[//]") as "H". simpl. iFrame.
-Qed.
+  iDestruct ("H" with "[//]") as "H". simpl. rewrite app_nil_r. iFrame.
+  
+Admitted.
 
-Lemma wp_lift_pure_stuck `{!Inhabited (state Λ)} E Φ e :
+Lemma wp_lift_pure_stuck `{!Inhabited (state Λ)} E Φ e i :
   (∀ σ, stuck e σ) →
-  True ⊢ WP e @ E ?{{ Φ }}.
+  True ⊢ WP e @ (MaybeStuck,i); E {{ Φ }}.
 Proof.
   iIntros (Hstuck) "_". iApply wp_lift_stuck.
   - destruct(to_val e) as [v|] eqn:He; last done.
@@ -85,18 +86,18 @@ Qed.
 
 (* Atomic steps don't need any mask-changing business here, one can
    use the generic lemmas here. *)
-Lemma wp_lift_atomic_step_fupd {s E1 E2 Φ} e1 :
+Lemma wp_lift_atomic_step_fupd {s i E1 E2 Φ} e1 :
   to_val e1 = None →
-  (∀ σ1 κ κs n, state_interp σ1 (κ ++ κs) n ={E1}=∗
+  (∀ σ1 κ κs es K, state_interp σ1 (κ ++ κs) es ={E1}=∗
     ⌜if s is NotStuck then reducible e1 σ1 ∨ waiting e1 σ1 else True⌝ ∗
     ∀ e2 σ2 efs, ⌜prim_step e1 σ1 κ e2 σ2 efs⌝ ={E1,E2}▷=∗
-      state_interp σ2 κs (length efs + n) ∗
+      state_interp σ2 κs ((<[i := fill K e2]> es) ++ efs) ∗
       from_option Φ False (to_val e2) ∗
-      [∗ list] ef ∈ efs, WP ef @ s; ⊤ {{ fork_post }})
-  ⊢ WP e1 @ s; E1 {{ Φ }}.
+      [∗ list] i ↦ ef ∈ efs, WP ef @ (s,length es + i); ⊤ {{ fork_post }})
+  ⊢ WP e1 @ (s,i); E1 {{ Φ }}.
 Proof.
   iIntros (?) "H".
-  iApply (wp_lift_step_fupd s E1 _ e1)=>//; iIntros (σ1 κ κs n) "Hσ1".
+  iApply (wp_lift_step_fupd s i E1 _ e1) =>//; iIntros (σ1 κ κs es K) "Hσ1".
   iMod ("H" $! σ1 with "Hσ1") as "[$ H]".
   iMod (fupd_intro_mask' E1 ∅) as "Hclose"; first set_solver.
   iIntros "!>" (e2 σ2 efs ?). iMod "Hclose" as "_".
@@ -107,18 +108,18 @@ Proof.
   iApply wp_value; last done. by apply of_to_val.
 Qed.
 
-Lemma wp_lift_atomic_step {s E Φ} e1 :
+Lemma wp_lift_atomic_step {s i E Φ} e1 :
   to_val e1 = None →
-  (∀ σ1 κ κs n, state_interp σ1 (κ ++ κs) n ={E}=∗
+  (∀ σ1 κ κs es K, state_interp σ1 (κ ++ κs) es ={E}=∗
     ⌜if s is NotStuck then reducible e1 σ1 ∨ waiting e1 σ1 else True⌝ ∗
     ▷ ∀ e2 σ2 efs, ⌜prim_step e1 σ1 κ e2 σ2 efs⌝ ={E}=∗
-      state_interp σ2 κs (length efs + n) ∗
+      state_interp σ2 κs ((<[i := fill K e2]> es) ++ efs) ∗
       from_option Φ False (to_val e2) ∗
-      [∗ list] ef ∈ efs, WP ef @ s; ⊤ {{ fork_post }})
-  ⊢ WP e1 @ s; E {{ Φ }}.
+      [∗ list] i ↦ ef ∈ efs, WP ef @ (s,length es + i); ⊤ {{ fork_post }})
+  ⊢ WP e1 @ (s,i); E {{ Φ }}.
 Proof.
   iIntros (?) "H". iApply wp_lift_atomic_step_fupd; [done|].
-  iIntros (????) "?". iMod ("H" with "[$]") as "[$ H]".
+  iIntros (?????) "?". iMod ("H" with "[$]") as "[$ H]".
   iIntros "!> *". iIntros (Hstep) "!> !>".
   by iApply "H".
 Qed.
